cfi/cfi_refinement.v
@@ -351,4 +351,52 @@ Proof.
     rewrite CLST. reflexivity.
 Qed.   
 
+(*Preservation Theorem*)
+
+Theorem backwards_refinement_preserves_cfi :
+  cfi amachine AS ->
+  cfi cmachine CS. 
+Proof. 
+  intros CFI1 cst cst' cxs INIT2 INTERM2.
+  destruct (initial_refine cst INIT2) as [ast [INIT1 INITREF]].
+  destruct (backwards_refinement_traces_stronger ast INITREF INTERM2)
+    as [axs [[ast' INTERMR1] RTRACE]].
+  destruct (intermr_implies_interm INTERMR1) as [INTERM1 | [EQ LST]].
+  { (*machine1  steps*)
+    clear INTERMR1.
+    destruct (CFI1 ast ast' axs INIT1 INTERM1) as [TSAFE1 | VIOLATED].
+    - (*machine1 has CFI at all steps*)
+      left. apply (refine_traces_preserves_cfi_trace RTRACE TSAFE1).
+    - (*machine1 has a violation*)
+      destruct VIOLATED 
+         as [asi [asj [ahs [atl [ALST [[ASTEP AV] [TSAFE1 [TSAFE2 STOP1]]]]]]]].
+      right.
+      assert (IN2: In2 asi asj axs) by (rewrite ALST; apply in2_trivial).
+      destruct (refine_traces_split ahs atl asi asj ALST RTRACE ASTEP AV) 
+        as [chs [csi [csj [ctl [CSTEP [VIS [REFI [REFJ [RHT [RTT CLST]]]]]]]]]].
+      exists csi; exists csj; exists chs; exists ctl.
+      split. now assumption.
+      split. split; [assumption | apply (av_implies_cv asi asj csi csj REFI REFJ AV VIS)].
+      split. now apply (refine_traces_preserves_cfi_trace RHT TSAFE1).
+      split. now apply (refine_traces_preserves_cfi_trace  RTT TSAFE2).
+      apply (as_implies_cs RTT STOP1).
+  }
+  { (*machine1 no step*)
+    subst. left.
+    intros csi csj IN2 CSTEP.
+    simpl in INTERMR1; apply intermr_first_step in INTERMR1; subst.
+    destruct cxs. inversion INTERM2.
+    apply interm_first_step in INTERM2; subst.
+    clear INIT1. clear INIT2. clear INITREF.
+    generalize dependent cst.
+    induction cxs; intros.
+    - destruct IN2.
+    - destruct IN2 as [[? ?] | IN2]; subst.
+      * inversion RTRACE; subst.
+        apply (cfg_invisible _ _ H4 H5).
+      * inversion RTRACE; subst.
+        now apply (IHcxs _ H8 IN2). 
+  }
+Qed.
+
 End Refinement.
